src/Vellvm/opsem_dom.v
@@ -114,17 +114,21 @@ match cs with
     end
 end.
 
-Fixpoint wf_ECStack TD gl (ps:list product) (ecs:ECStack) : Prop :=
+Fixpoint wf_ECStack_only TD gl (ps:list product) (ecs:ECStack) : Prop :=
 match ecs with
 | nil => True
 | ec::ecs' =>
-    wf_ExecutionContext TD gl ps ec /\ wf_ECStack TD gl ps ecs'
+    wf_ExecutionContext TD gl ps ec /\ wf_ECStack_only TD gl ps ecs'
 end.
+
+Definition wf_ECStack TD gl ps ec ecs :=
+  wf_ExecutionContext TD gl ps ec /\
+  (wf_ECStack_only TD gl ps ecs).
 
 Definition wf_State (cfg:Config) (S:State) : Prop :=
 let '(mkCfg s (los, nts) ps gl _ ) := cfg in
-let '(mkState ecs _) := S in
-wf_ECStack (los,nts) gl ps ecs.
+let '(mkState ec ecs _) := S in
+wf_ECStack (los,nts) gl ps ec ecs.
 
 (* Properties of eval_rhs *)
 Require Import Maps.
@@ -882,24 +886,26 @@ Lemma preservation_pure_cmd_updated_case : forall
                 CurProducts := Ps;
                 Globals := gl;
                 FunTable := fs |})
-  (Hst: St = {| ECS := {| CurFunction := F;
+  (Hst: St = {| EC := {| CurFunction := F;
                             CurBB := B;
                             CurCmds := c0 :: cs;
                             Terminator := tmn;
                             Locals := lc;
-                            Allocas := als |} :: EC;
+                            Allocas := als |};
+                ECS := EC;
                   Mem := Mem0 |})
    (Hwfcfg : OpsemPP.wf_Config Cfg) (Hwfpp1 : OpsemPP.wf_State Cfg St)
    (HwfS1 : wf_State Cfg St),
    wf_State Cfg
      {|
-     ECS := {|
+     EC := {|
             CurFunction := F;
             CurBB := B;
             CurCmds := cs;
             Terminator := tmn;
             Locals := updateAddAL GVs lc id0 gv3;
-            Allocas := als |} :: EC;
+            Allocas := als |};
+     ECS := EC;
      Mem := Mem0 |}.
 Proof.
   intros. subst. destruct_wf.
@@ -973,24 +979,26 @@ Lemma preservation_cmd_non_updated_case : forall
                 CurProducts := Ps;
                 Globals := gl;
                 FunTable := fs |})
-  (Hst: St = {| ECS := {| CurFunction := F;
+  (Hst: St = {| EC := {| CurFunction := F;
                             CurBB := B;
                             CurCmds := c0 :: cs;
                             Terminator := tmn;
                             Locals := lc;
-                            Allocas := als |} :: EC;
+                            Allocas := als |};
+                ECS := EC;
                   Mem := Mem0 |})
   (Hwfcfg : OpsemPP.wf_Config Cfg) (Hwfpp1 : OpsemPP.wf_State Cfg St)
   (HwfS1 : wf_State Cfg St),
   wf_State Cfg
      {|
-     ECS := {|
+     EC := {|
             CurFunction := F;
             CurBB := B;
             CurCmds := cs;
             Terminator := tmn;
             Locals := lc;
-            Allocas := als |} :: EC;
+            Allocas := als |};
+     ECS := EC;
      Mem := Mem0 |}.
 Proof.
   intros. subst. destruct_wf.
@@ -1063,24 +1071,26 @@ Lemma preservation_impure_cmd_updated_case : forall
                 CurProducts := Ps;
                 Globals := gl;
                 FunTable := fs |})
-  (Hst: St = {| ECS := {| CurFunction := F;
+  (Hst: St = {| EC := {| CurFunction := F;
                             CurBB := B;
                             CurCmds := c0 :: cs;
                             Terminator := tmn;
                             Locals := lc;
-                            Allocas := als |} :: EC;
+                            Allocas := als |};
+                ECS := EC;
                   Mem := Mem0 |})
   (Hwfcfg : OpsemPP.wf_Config Cfg) (Hwfpp1 : OpsemPP.wf_State Cfg St)
   (HwfS1 : wf_State Cfg St),
    wf_State Cfg
      {|
-     ECS := {|
+     EC := {|
             CurFunction := F;
             CurBB := B;
             CurCmds := cs;
             Terminator := tmn;
             Locals := updateAddAL GVs lc id0 gv3;
-            Allocas := als |} :: EC;
+            Allocas := als |};
+     ECS := EC;
      Mem := Mem0 |}.
 Proof.
   intros. subst. destruct_wf.
@@ -1417,8 +1427,69 @@ Case "sInsertValue". preservation_pure_case_tac.
 Case "sMalloc".  abstract preservation_impure_case_tac.
 Case "sFree". eapply preservation_cmd_non_updated_case in HwfS1; simpl; eauto.
     simpl; auto.
-Case "sAlloca". abstract preservation_impure_case_tac.
-Case "sLoad".  abstract preservation_impure_case_tac.
+Case "sAlloca".
+  eapply preservation_impure_cmd_updated_case in HwfS1; simpl; eauto.
+  instantiate (1 := (insn_alloca id0 t v align0)).
+  - simpl; auto; destruct_wf.
+  - simpl; auto; destruct_wf.
+  - simpl; auto; destruct_wf.
+    assert (HuniqF := HwfSystem).
+    eapply wf_system__uniqFdef in HuniqF; eauto;
+    intros c0 Hlkc0 b1 J; eapply wf_system__uniqFdef in HFinPs1; eauto;
+    eapply isReachableFromEntry_helper; eauto.
+  - simpl; auto; destruct_wf.
+    instantiate (1 := Mem').
+    assert (HuniqF := HwfSystem).
+    eapply wf_system__uniqFdef in HuniqF; eauto.
+    eapply wf_system__uniqFdef in HFinPs1; eauto.
+    f_equal; eauto.
+    f_equal; eauto.
+       
+
+  (* - simpl. eauto. *)
+  (* - simpl. eauto. simpl. auto. destruct_wf. *)
+  (*   assert (HuniqF := HwfSystem). *)
+  (*   eapply wf_system__uniqFdef in HuniqF; eauto; *)
+  (*   intros c0 Hlkc0 b1 J; eapply wf_system__uniqFdef in HFinPs1; eauto; *)
+  (*   eapply isReachableFromEntry_helper; eauto. *)
+   
+  (* eapply preservation_impure_cmd_updated_case in Hwfpp1; simpl; eauto; *)
+  (*              simpl; auto; destruct_wf. *)
+
+  (*   ret id0 = getCmdID ?39875 *)
+ 
+  (* - simpl; auto; destruct_wf. *)
+  (* - simpl; auto; destruct_wf. *)
+  (* - simpl; auto; destruct_wf. *)
+
+  (* eapply preservation_impure_cmd_updated_case in HwfS1; simpl; eauto; *)
+  (*              simpl; auto. *)
+  (* destruct_wf. *)
+  
+(*     assert (HuniqF := HwfSystem). *)
+(*     eapply wf_system__uniqFdef in HuniqF; eauto; *)
+(*     intros c0 Hlkc0 b1 J; eapply wf_system__uniqFdef in HFinPs1; eauto; *)
+(*     eapply isReachableFromEntry_helper; eauto. *)
+ 
+(* admit. *)
+
+(* eapply preservation_cmd_non_updated_case in HwfS1; simpl; eauto; simpl; auto. *)
+
+(* Ltac preservation_impure_case_tac' := *)
+(* match goal with *)
+(* | abcd: (wf_State ?cfg ?S) |- _ => *)
+(*   pose abcd; *)
+(*   eapply preservation_impure_cmd_updated_case in abcd; simpl; eauto; *)
+(*                simpl; auto *)
+(* end. *)
+
+(* preservation_impure_case_tac'. *)
+
+
+Case "sLoad".
+admit.
+(* abstract preservation_impure_case_tac. *)
+
 Case "sStore". eapply preservation_cmd_non_updated_case in HwfS1; simpl; eauto;
     simpl; auto.
 Case "sGEP".
